src/OptimisticFSSpecs.v
@@ -1,0 +1,90 @@
+Require Import CCL.
+Require Import Hashmap.
+
+Require Import OptimisticFS.
+Require Import FSProtocol.
+
+Import BFile.
+Import OptimisticCache.
+
+Record FsSpecParams T :=
+  { fs_pre : dirtree -> Prop;
+    fs_post : T -> Prop;
+    fs_dirup : dirtree -> dirtree; }.
+
+Definition FsSpec A T := A -> FsSpecParams T.
+
+Section FsSpecs.
+
+  Variable P:FsParams.
+
+  Definition fs_spec A T (fsspec: FsSpec A T) tid :
+    memstate -> LocalLock -> Cache ->
+    Spec _ (Result (memstate * T) * Cache) :=
+    fun mscs l c '(F, d, vd, tree, a) sigma =>
+      {| precondition :=
+           F (Sigma.mem sigma) /\
+           cache_rep d c vd /\
+           (l = Locked -> d = Sigma.disk sigma) /\
+           fs_rep P vd (Sigma.hm sigma) mscs tree /\
+           fs_pre (fsspec a) tree /\
+           local_l tid (Sigma.l sigma) = l;
+         postcondition :=
+           fun sigma' '(r, c') =>
+             exists vd',
+               F (Sigma.mem sigma') /\
+               translated_postcondition l d sigma c vd sigma' c' vd' /\
+               match r with
+               | Success _ (mscs', r) =>
+                 fs_post (fsspec a) r /\
+                 fs_rep P vd' (Sigma.hm sigma') mscs' (fs_dirup (fsspec a) tree)
+               | Failure e =>
+                 (l = Locked -> e <> WriteRequired) /\
+                 vd = vd' /\
+                 fs_rep P vd' (Sigma.hm sigma') mscs tree
+               end /\
+               hashmap_le (Sigma.hm sigma) (Sigma.hm sigma') ; |}.
+
+  Lemma translated_post_hashmap_le : forall l d sigma c vd sigma' c' vd',
+      translated_postcondition l d sigma c vd sigma' c' vd' ->
+      hashmap_le (Sigma.hm sigma) (Sigma.hm sigma').
+  Proof.
+    unfold translated_postcondition; intuition.
+  Qed.
+
+  Hint Resolve translated_post_hashmap_le.
+
+  Ltac finish :=
+    repeat (split; [ | solve [ trivial ] ]);
+    descend; simpl in *; subst;
+    intuition (try eassumption; eauto).
+
+  Hint Extern 1 {{ OptFS.file_get_attr _ _ _ _ _; _ }} => apply OptFS.file_get_attr_ok : prog.
+
+  Theorem opt_file_get_attr_ok : forall G inum mscs l tid c,
+      cprog_spec G tid
+                 (fs_spec (fun '(pathname, f) =>
+                             {| fs_pre :=
+                                  fun tree => find_subtree pathname tree = Some (TreeFile inum f);
+                                fs_post :=
+                                  fun '(r, _) => r = BFILE.BFAttr f;
+                                fs_dirup := fun tree => tree |}) tid mscs l c)
+                 (OptFS.file_get_attr (fsxp P) inum mscs l c).
+  Proof using Type.
+    unfold fs_spec; intros.
+    step; simpl in *; safe_intuition.
+    unfold Prog.pair_args_helper in *.
+    match goal with
+    | [ H: fs_rep _ _ _ _ _ |- _ ] =>
+      unfold fs_rep in H; simplify
+    end.
+    destruct frees; finish.
+    SepAuto.pred_apply; SepAuto.cancel; eauto.
+
+    step; finish.
+    destruct_goal_matches; SepAuto.destruct_lifts; finish.
+    unfold fs_rep; finish.
+    eapply fs_rep_hashmap_incr; unfold fs_rep; finish.
+  Qed.
+
+End FsSpecs.
